finish union_insert

coq/st/left/union_insert.v
@@ -48,6 +48,7 @@ which is not correct.
 
 Approach 3
 ----------
+??? 
 
 *) 
 Require Import Coq.Strings.String.
@@ -57,7 +58,9 @@ Require Import CAS.coq.eqv.properties.
 Require Import CAS.coq.eqv.structures. 
 Require Import CAS.coq.eqv.set.
 Require Import CAS.coq.eqv.add_constant.
-Require Import CAS.coq.eqv.sum. 
+Require Import CAS.coq.eqv.sum.
+Require Import CAS.coq.sg.properties. 
+Require Import CAS.coq.sg.structures.
 Require Import CAS.coq.sg.union.
 Require Import CAS.coq.sg.cast_up.
 Require Import CAS.coq.sg.add_ann. 
@@ -150,20 +153,26 @@ End Theory.
 
 Section ACAS.
 
-(*
-Definition union_insert_left_semiring_proofs (S : Type) (eq : brel S) (wS : S) (eqvP : eqv_proofs S eq) :=
+Definition union_insert_slt_proofs
+           (S : Type)
+           (c : cas_constant)
+           (eq : brel S)
+           (wS : S)
+           (f : S → S)
+           (nt : brel_not_trivial S eq f) 
+           (eqvP : eqv_proofs S eq) :=
 let ref := A_eqv_reflexive _ _ eqvP in
 let sym := A_eqv_symmetric _ _ eqvP in
 let trn := A_eqv_transitive _ _ eqvP in      
 {|
-  A_left_semiring_distributive   := @slt_union_insert_distributive S eq ref sym trn 
-; A_left_semiring_not_absorptive := @slt_union_insert_not_absorptive S wS eq 
+  A_slt_distributive_d   := inr (slt_union_insert_not_distributive S c wS eq f nt ref sym trn)
+; A_slt_absorptive_d := inr (slt_union_insert_not_absorptive S c wS eq)
+; A_slt_strictly_absorptive_d := inr (slt_union_insert_not_strictly_absorptive S c wS eq)
 |}.
 
 Open Scope string_scope.
 
-
-Definition A_slt_union_insert (S :Type) (eqv : A_eqv S) :=
+Definition A_slt_union_insert (S :Type) (eqv : A_eqv S) (c : cas_constant) :=
 let eq         := A_eqv_eq S eqv in
 let wS          := A_eqv_witness S eqv in
 let f          := A_eqv_new S eqv in
@@ -174,25 +183,35 @@ let refS       := A_eqv_reflexive _ _ eqvP in
 let symS       := A_eqv_symmetric _ _ eqvP in
 let trnS       := A_eqv_transitive _ _ eqvP in
   {|
-    A_left_pre_semiring_carrier           := A_eqv_set S eqv 
-  ; A_left_pre_semiring_label             := eqv 
-  ; A_left_pre_semiring_plus              := bop_union eq 
-  ; A_left_pre_semiring_trans             := ltr_insert eq 
-  ; A_left_pre_semiring_plus_proofs       := (* ugh!  need some abstraction here....*)
-                                             A_sg_C_proofs_from_sg_CI_proofs
-                                               (finite_set S) 
-                                               (brel_set eq)
-                                               (bop_union eq) 
-                                               (wS :: nil)
-                                               (λ (l : finite_set S), if brel_set eq nil l then (wS :: nil) else nil)
-                                               (brel_set_not_trivial S eq wS)
-                                               (eqv_proofs_set S eq eqvP)
-                                               (sg_CI_proofs_union eqv)
-  ; A_left_pre_semiring_trans_proofs      := ltr_insert_proofs S eq wS f ntS eqvP 
-  ; A_left_pre_semiring_exists_plus_ann_d := bop_union_exists_ann_decide S eq refS symS trnS fin_d 
-  ; A_left_pre_semiring_id_ann_proofs_d   := slt_union_insert_exists_id_ann_decide S wS eq refS symS trnS fin_d 
-  ; A_left_pre_semiring_proofs            := union_insert_left_semiring_proofs S eq wS eqvP  
-  ; A_left_pre_semiring_ast               := Cas_ast ("slt_union_insert", (Cas_eqv_ast (A_eqv_ast _ eqv)) :: nil)
+    A_slt_carrier           := A_eqv_add_constant _ (A_eqv_set S eqv) c 
+  ; A_slt_label             := eqv 
+  ; A_slt_plus              := bop_add_ann (bop_union eq) c 
+  ; A_slt_trans             := ltr_insert eq 
+  ; A_slt_plus_proofs       :=
+      (* triple UGLY!  need some abstraction here.... FIX someday .... *) 
+      sg_proofs_add_ann
+        (finite_set S)
+        (brel_set eq)
+        c
+        (bop_union eq)
+        (wS :: nil)
+        (λ (l : finite_set S), if brel_set eq nil l then (wS :: nil) else nil)
+        (brel_set_not_trivial S eq wS)
+        (eqv_proofs_set S eq eqvP)
+        (A_sg_proofs_from_sg_CI_proofs
+           (finite_set S) 
+           (brel_set eq)
+           (bop_union eq) 
+           (wS :: nil)
+           (λ (l : finite_set S), if brel_set eq nil l then (wS :: nil) else nil)
+           (brel_set_not_trivial S eq wS)
+           (eqv_proofs_set S eq eqvP)
+           (sg_CI_proofs_union eqv))
+  ; A_slt_trans_proofs      := ltr_insert_proofs S eq wS f ntS eqvP 
+  ; A_slt_exists_plus_ann_d := inl (bop_add_ann_exists_ann _ (brel_set eq) c (bop_union eq))
+  ; A_slt_id_ann_proofs_d   := slt_union_insert_exists_id_ann_decide S c wS eq refS symS trnS fin_d 
+  ; A_slt_proofs            := union_insert_slt_proofs S c eq wS f ntS eqvP  
+  ; A_slt_ast               := Cas_ast ("slt_union_insert", (Cas_eqv_ast (A_eqv_ast S eqv)) :: (Cas_ast_constant c) :: nil)
 |}.
 
  
@@ -201,9 +220,9 @@ End ACAS.
 Section AMCAS.
 
 
-Definition A_mcas_slt_union_insert (S : Type) (eqv : @A_mcas_eqv S) :=
+Definition A_mcas_slt_union_insert (S : Type) (eqv : @A_mcas_eqv S) (c : cas_constant) :=
 match eqv with
-| A_EQV_eqv A    => A_slt_classify (A_SLT_Left_Pre_Semiring (A_slt_union_insert _ A))
+| A_EQV_eqv A    => A_slt_classify (A_SLT (A_slt_union_insert _ A c))
 | A_EQV_Error sl => A_SLT_Error sl     
 end.
   
@@ -211,55 +230,63 @@ End AMCAS.
 
 Section CAS.
 
-Definition union_insert_left_semiring_certs {S : Type} (wS : S) :=
+Definition union_insert_slt_certs {S : Type} (c : cas_constant) (wS : S) (f : S -> S) :=
 {|
-  left_semiring_distributive   := Assert_Slt_Distributive 
-; left_semiring_not_absorptive := @Assert_Slt_Not_Absorptive S (finite_set S) (wS, nil) 
+  slt_distributive_d        := @Certify_Slt_Not_Distributive S (with_constant (finite_set S)) (wS, (inl c, inr ((f wS) :: nil)))
+; slt_absorptive_d          := @Certify_Slt_Not_Absorptive S (with_constant (finite_set S)) (wS, inr nil)
+; slt_strictly_absorptive_d := @Certify_Slt_Not_Strictly_Absorptive S (with_constant (finite_set S)) (wS, inr nil)
 |}.
 
 Open Scope string_scope.
 
 
-Definition slt_union_insert_exists_id_ann_certify {S : Type} (fin_d : @check_is_finite S) : @check_slt_exists_id_ann S (finite_set S) :=
+Definition slt_union_insert_exists_id_ann_certify
+           {S : Type}
+           (fin_d : @check_is_finite S) : @check_slt_exists_id_ann S (with_constant (finite_set S)) :=
   match fin_d with
-  | Certify_Is_Finite enum => Certify_SLT_Id_Ann_Proof_Not_Equal (nil, enum tt)
-  | Certify_Is_Not_Finite  => Certify_SLT_Id_Ann_Proof_Id_None nil 
-  end. 
+  | Certify_Is_Finite enum => Certify_SLT_Id_Ann_Proof_Not_Equal (inr nil, inr (enum tt))
+  | Certify_Is_Not_Finite  => Certify_SLT_Id_Ann_Proof_Id_None (inr nil) 
+  end.
+
   
-Definition slt_union_insert {S :Type} (eqv : @eqv S) :=
+Definition slt_union_insert {S :Type} (eqv : @eqv S) (c : cas_constant) :=
 let eq         := eqv_eq eqv in
 let wS         := eqv_witness eqv in
 let f          := eqv_new eqv in
 let fin_d      := eqv_finite_d eqv in
   {|
-    left_pre_semiring_carrier           := eqv_set eqv 
-  ; left_pre_semiring_label             := eqv 
-  ; left_pre_semiring_plus              := bop_union eq 
-  ; left_pre_semiring_trans             := ltr_insert eq 
-  ; left_pre_semiring_plus_certs        := (* ugh!  need some abstraction here....*)
-                                             sg_C_certs_from_sg_CI_certs
-                                               (finite_set S) 
-                                               (brel_set eq)
-                                               (bop_union eq) 
-                                               (wS :: nil)
-                                               (λ (l : finite_set S), if brel_set eq nil l then (wS :: nil) else nil)
-                                               (sg_CI_certs_union eqv)
-  ; left_pre_semiring_trans_certs       := ltr_insert_certs wS f 
-  ; left_pre_semiring_exists_plus_ann_d := bop_union_exists_ann_certify fin_d 
-  ; left_pre_semiring_id_ann_certs_d    := slt_union_insert_exists_id_ann_certify fin_d 
-  ; left_pre_semiring_certs             := union_insert_left_semiring_certs wS
-  ; left_pre_semiring_ast               := Cas_ast ("slt_union_insert", (Cas_eqv_ast (eqv_ast eqv)) :: nil)
+    slt_carrier           := eqv_add_constant (eqv_set eqv) c 
+  ; slt_label             := eqv 
+  ; slt_plus              := bop_add_ann (bop_union eq) c
+  ; slt_trans             := ltr_insert eq 
+  ; slt_plus_certs        :=
+      (* triple UGLY!  need some abstraction here.... FIX someday .... *) 
+      @sg_certs_add_ann 
+        (finite_set S)
+        c 
+        (wS :: nil)
+        (λ (l : finite_set S), if brel_set eq nil l then (wS :: nil) else nil)
+        (sg_certs_from_sg_CI_certs
+           (finite_set S) 
+           (brel_set eq)
+           (bop_union eq) 
+           (wS :: nil)
+           (λ (l : finite_set S), if brel_set eq nil l then (wS :: nil) else nil)
+           (sg_CI_certs_union eqv))
+  ; slt_trans_certs       := ltr_insert_certs wS f 
+  ; slt_exists_plus_ann_d := Certify_Exists_Ann  (inl c)                                  
+  ; slt_id_ann_certs_d    := slt_union_insert_exists_id_ann_certify fin_d 
+  ; slt_certs             := union_insert_slt_certs c wS f
+  ; slt_ast               := Cas_ast ("slt_union_insert", (Cas_eqv_ast (eqv_ast eqv)) :: (Cas_ast_constant c) :: nil)
 |}.
-
-  
   
 End CAS.
 
 Section MCAS.
 
-Definition mcas_slt_union_insert {S : Type} (eqv : @mcas_eqv S) :=
+Definition mcas_slt_union_insert {S : Type} (eqv : @mcas_eqv S) (c : cas_constant):=
 match eqv with
-| EQV_eqv A    => slt_classify (SLT_Left_Pre_Semiring (slt_union_insert A))
+| EQV_eqv A    => slt_classify (SLT (slt_union_insert A c))
 | EQV_Error sl => SLT_Error sl     
 end.
   
@@ -268,8 +295,27 @@ End MCAS.
 
 Section Verify.
 
+
+Lemma correct_certs_union_insert
+      (S : Type)
+      (c : cas_constant)
+      (eq : brel S)
+      (wS : S)
+      (f : S → S)
+      (nt : brel_not_trivial S eq f) 
+      (eqvP : eqv_proofs S eq) :    
+      union_insert_slt_certs c wS f 
+      = 
+      P2C_slt (brel_sum brel_constant (brel_set eq))
+              (bop_add_ann (bop_union eq) c)
+              (ltr_insert eq)
+              (union_insert_slt_proofs S c eq wS f nt eqvP). 
+Proof. compute. reflexivity. Qed. 
+  
+
 Lemma correct_id_ann_certs_union_insert
       (S : Type)
+      (c : cas_constant)
       (eq : brel S)
       (wS : S)
       (fin_d : carrier_is_finite_decidable S eq)
@@ -278,50 +324,50 @@ Lemma correct_id_ann_certs_union_insert
       (trn : brel_transitive S eq) : 
      slt_union_insert_exists_id_ann_certify (p2c_is_finite_check S eq fin_d)
      =
-     p2c_slt_exists_id_ann_check (brel_set eq) (bop_union eq) (ltr_insert eq)
-        (slt_union_insert_exists_id_ann_decide S wS eq ref sym trn fin_d). 
+     p2c_slt_exists_id_ann_check 
+        (brel_sum brel_constant (brel_set eq))
+        (bop_add_ann (bop_union eq) c) 
+        (ltr_insert eq)
+        (slt_union_insert_exists_id_ann_decide 
+            S c wS eq ref sym trn fin_d). 
 Proof. unfold p2c_slt_exists_id_ann_check, slt_union_insert_exists_id_ann_decide,
               slt_union_insert_exists_id_ann_certify, p2c_is_finite_check; 
               destruct fin_d as [[enum A] | C]; simpl; reflexivity. 
 Qed.
 
-Lemma correct_certs_union_insert (S : Type) (eq : brel S) (wS : S) (eqvP : eqv_proofs S eq) :    
-      union_insert_left_semiring_certs wS 
-      = 
-      P2C_left_semiring (brel_set eq) (bop_union eq) (ltr_insert eq)
-        (union_insert_left_semiring_proofs S eq wS eqvP). 
-Proof. unfold union_insert_left_semiring_certs,
-       union_insert_left_semiring_proofs,
-       P2C_left_semiring; compute.
-       reflexivity. 
-Qed. 
   
-Theorem correct_union_insert (S : Type) (eqv: A_eqv S) : 
-    slt_union_insert (A2C_eqv S eqv)
+Theorem correct_union_insert (S : Type) (eqv: A_eqv S) (c : cas_constant) : 
+    slt_union_insert (A2C_eqv S eqv) c
     =
-    A2C_left_pre_semiring (A_slt_union_insert S eqv).
-Proof. unfold slt_union_insert, A_slt_union_insert, A2C_left_pre_semiring; simpl.
-       rewrite correct_eqv_set.
+    A2C_slt (A_slt_union_insert S eqv c).
+Proof. unfold slt_union_insert, A_slt_union_insert, A2C_slt; simpl.
+       rewrite correct_eqv_set.       
+       rewrite correct_eqv_add_constant. 
+       rewrite correct_ltr_insert_certs.
+       rewrite <- correct_certs_union_insert.               
+       rewrite <- correct_id_ann_certs_union_insert.
+       (* UGLY! *)
+       unfold A_sg_proofs_from_sg_CI_proofs. 
+       unfold sg_certs_from_sg_CI_certs.
        rewrite correct_bop_union_certs.
-       rewrite correct_ltr_certs_insert. 
-       rewrite <- correct_bop_union_exists_ann_certify.
-       rewrite <- correct_id_ann_certs_union_insert.       
-       rewrite <- correct_certs_union_insert.        
-       rewrite <- correct_sg_C_certs_from_sg_CI_certs.
-
+       rewrite <- correct_sg_certs_add_ann.
+       rewrite <- correct_sg_certs_from_sg_C_certs.       
+       rewrite <- correct_sg_C_certs_from_sg_CI_certs.              
        reflexivity.
 Qed. 
 
  
-Theorem correct_bop_mcas_union_insert (S : Type) (eqvS : @A_mcas_eqv S): 
-         mcas_slt_union_insert (A2C_mcas_eqv S eqvS)  
+Theorem correct_bop_mcas_union_insert (S : Type) (eqvS : @A_mcas_eqv S) (c : cas_constant): 
+         mcas_slt_union_insert (A2C_mcas_eqv S eqvS) c
          = 
-         A2C_mcas_slt (A_mcas_slt_union_insert S eqvS). 
-Proof. destruct eqvS; simpl.
-       + reflexivity. 
+         A2C_mcas_slt (A_mcas_slt_union_insert S eqvS c). 
+Proof. unfold mcas_slt_union_insert, A_mcas_slt_union_insert.
+       unfold A_slt_classify, slt_classify.       
+       destruct eqvS; unfold A2C_mcas_eqv. 
+       + simpl. reflexivity. 
        + rewrite correct_union_insert.
-         apply correctness_slt_classify_left_pre_semiring_slt. 
+         rewrite <- correctness_slt_classify_slt.
+         reflexivity. 
 Qed.  
 
 End Verify.   
-*) 
